fairness/lawyer/obligations/obls_termination.v
@@ -1,0 +1,54 @@
+From iris.proofmode Require Import tactics.
+From iris.algebra Require Import gset gmultiset.
+From trillium.fairness Require Import locales_helpers inftraces fairness.
+From trillium.fairness.lawyer.obligations Require Import obligations_model.
+
+
+Section Termination.
+  Context `(OP: ObligationsParams Degree Level Locale LIM_STEPS).
+  Context `{Countable Locale}. 
+  Let OM := ObligationsModel OP.
+
+
+  Section NoInfExpects.
+    Context (tr: obls_trace OP).
+    Context {last_expect: SignalId -> nat}.
+    Hypothesis (LAST_EXP_SPEC: 
+                 forall sid δ1 δ2 τ k π d,
+                   tr !! k = Some (δ1, Some (τ, δ2)) ->
+                   expects_ep OP δ1 τ δ2 sid π d -> 
+                   k <= last_expect sid).
+
+    Definition PF (i: nat): gmultiset (@CallPermission Degree) :=
+      from_option (ps_cps OP) ∅ (tr S!! i) ⊎
+      (* ([^op set] ('(s, (π, d)) ∈ (∅: gset ExpectPermission)), ∅).  *)
+      ([^op set] ep ∈ (∅: gset (@ExpectPermission Degree)),
+        let '(sid, π, d) := ep in 
+        (last_expect sid - i) *: {[+ (π, d) +]}
+      ).
+
+    (* TODO: move into ObligationsParams *)
+    Context (deg_le: relation Degree). 
+    Context (DEG_PO: PartialOrder deg_le).
+
+    Definition cp_le: relation (@CallPermission Degree) :=
+      (* lexprod *)
+      fun '(_, d1) '(_, d2) => deg_le d1 d2.
+
+    (** TODO:
+        1) do we need to care about phases?
+        2) how to implement comparison of CPs multisets?
+     *)
+   
+  End NoInfExpects.
+
+  Lemma obls_fair_trace_terminate (tr: obls_trace OP):
+    obls_trace_valid OP tr ->
+    (∀ τ, obls_trace_fair OP τ tr) ->
+    terminating_trace tr.
+  Proof using.
+    
+  Admitted. 
+
+
+End Termination.
